Phi_System/IDE_CP_Reasoning3.thy
@@ -487,39 +487,6 @@ lemma [\<phi>reason 3200]:
   for X :: \<open>'a::sep_magma_1 set\<close>
   unfolding mult_1_right .
 
-subsection \<open>Pad Void Holes at left\<close> \<comment> \<open>to standardize\<close>
-
-lemma [\<phi>reason 2500
- except \<open> ?H \<^bold>i\<^bold>m\<^bold>p\<^bold>l\<^bold>i\<^bold>e\<^bold>s \<blangle> (?X1 * ?X2) \<brangle> \<^bold>a\<^bold>n\<^bold>d ?P @action reason_ToSA ?mode ?G\<close>
-        \<open> ?H \<^bold>i\<^bold>m\<^bold>p\<^bold>l\<^bold>i\<^bold>e\<^bold>s \<blangle> ?X1 + ?X2 \<brangle> \<^bold>a\<^bold>n\<^bold>d ?P @action reason_ToSA ?mode ?G\<close>
-        \<open> ?H \<^bold>i\<^bold>m\<^bold>p\<^bold>l\<^bold>i\<^bold>e\<^bold>s \<blangle> 1 \<brangle> \<^bold>a\<^bold>n\<^bold>d ?P @action reason_ToSA ?mode ?G\<close>
-        \<open> ?H \<^bold>i\<^bold>m\<^bold>p\<^bold>l\<^bold>i\<^bold>e\<^bold>s \<blangle> TAIL ?X \<brangle> \<^bold>a\<^bold>n\<^bold>d ?P @action reason_ToSA ?mode ?G\<close>
-]:
-  " H \<^bold>i\<^bold>m\<^bold>p\<^bold>l\<^bold>i\<^bold>e\<^bold>s \<blangle> 1 * X \<brangle> \<^bold>a\<^bold>n\<^bold>d P @action reason_ToSA mode G \<Longrightarrow>
-    H \<^bold>i\<^bold>m\<^bold>p\<^bold>l\<^bold>i\<^bold>e\<^bold>s \<blangle> X \<brangle> \<^bold>a\<^bold>n\<^bold>d P @action reason_ToSA mode G"
-  for X :: \<open>'a::sep_magma_1 set\<close>
-  unfolding mult_1_left .
-
-lemma [\<phi>reason 2500
-   except \<open> ?Y1 * ?Y2 \<^bold>i\<^bold>m\<^bold>p\<^bold>l\<^bold>i\<^bold>e\<^bold>s ?X \<^bold>a\<^bold>n\<^bold>d ?P @action reason_ToSA ?mode ?G\<close>
-          \<open> ?Y1 + ?Y2 \<^bold>i\<^bold>m\<^bold>p\<^bold>l\<^bold>i\<^bold>e\<^bold>s ?X \<^bold>a\<^bold>n\<^bold>d ?P @action reason_ToSA ?mode ?G\<close>
-          \<open> 1 \<^bold>i\<^bold>m\<^bold>p\<^bold>l\<^bold>i\<^bold>e\<^bold>s ?X \<^bold>a\<^bold>n\<^bold>d ?P @action reason_ToSA ?mode ?G\<close>
-          \<open> TAIL ?H \<^bold>i\<^bold>m\<^bold>p\<^bold>l\<^bold>i\<^bold>e\<^bold>s ?X \<^bold>a\<^bold>n\<^bold>d ?P @action reason_ToSA ?mode ?G\<close>
-]:
-  " 1 * Y \<^bold>i\<^bold>m\<^bold>p\<^bold>l\<^bold>i\<^bold>e\<^bold>s X \<^bold>a\<^bold>n\<^bold>d P @action reason_ToSA mode G \<Longrightarrow>
-    Y \<^bold>i\<^bold>m\<^bold>p\<^bold>l\<^bold>i\<^bold>e\<^bold>s X \<^bold>a\<^bold>n\<^bold>d P @action reason_ToSA mode G"
-  for X :: \<open>'a::sep_magma_1 set\<close>
-  unfolding mult_1_left .
-
-
-lemma [\<phi>reason 1050 for \<open>?X \<^bold>i\<^bold>m\<^bold>p\<^bold>l\<^bold>i\<^bold>e\<^bold>s \<blangle> ?Y \<brangle> \<^bold>a\<^bold>n\<^bold>d ?P @action reason_ToSA True ?G\<close>
-   except \<open>(?X'::?'a::sep_magma_1 set) \<^bold>i\<^bold>m\<^bold>p\<^bold>l\<^bold>i\<^bold>e\<^bold>s \<blangle> ?Y' \<brangle> \<^bold>a\<^bold>n\<^bold>d ?P @action reason_ToSA True ?G\<close>]:
-  \<open> X \<^bold>i\<^bold>m\<^bold>p\<^bold>l\<^bold>i\<^bold>e\<^bold>s Y \<^bold>a\<^bold>n\<^bold>d P
-\<Longrightarrow> X \<^bold>i\<^bold>m\<^bold>p\<^bold>l\<^bold>i\<^bold>e\<^bold>s \<blangle> Y \<brangle> \<^bold>a\<^bold>n\<^bold>d P @action reason_ToSA True G\<close>
-  \<comment> \<open>If it doesn't have one, it cannot be reasoned by this procedure, so
-      a fallback here handles it.\<close>
-  unfolding FOCUS_TAG_def Action_Tag_def .
-
 
 subsection \<open>Subjection\<close>
 
@@ -791,6 +758,36 @@ hide_fact ToSA_cond_target_A' ToSA_cond_target_B'
 
 subsection \<open>Step-by-Step Searching Procedure\<close>
 
+lemma [\<phi>reason 2100
+ except \<open> ?H \<^bold>i\<^bold>m\<^bold>p\<^bold>l\<^bold>i\<^bold>e\<^bold>s \<blangle> (?X1 * ?X2) \<brangle> \<^bold>a\<^bold>n\<^bold>d ?P @action reason_ToSA ?mode ?G\<close>
+        \<open> ?H \<^bold>i\<^bold>m\<^bold>p\<^bold>l\<^bold>i\<^bold>e\<^bold>s \<blangle> 1 \<brangle> \<^bold>a\<^bold>n\<^bold>d ?P @action reason_ToSA ?mode ?G\<close>
+        \<open> ?H \<^bold>i\<^bold>m\<^bold>p\<^bold>l\<^bold>i\<^bold>e\<^bold>s \<blangle> TAIL ?X \<brangle> \<^bold>a\<^bold>n\<^bold>d ?P @action reason_ToSA ?mode ?G\<close>
+]:
+  " H \<^bold>i\<^bold>m\<^bold>p\<^bold>l\<^bold>i\<^bold>e\<^bold>s \<blangle> 1 * X \<brangle> \<^bold>a\<^bold>n\<^bold>d P @action reason_ToSA mode G \<Longrightarrow>
+    H \<^bold>i\<^bold>m\<^bold>p\<^bold>l\<^bold>i\<^bold>e\<^bold>s \<blangle> X \<brangle> \<^bold>a\<^bold>n\<^bold>d P @action reason_ToSA mode G"
+  for X :: \<open>'a::sep_magma_1 set\<close>
+  unfolding mult_1_left .
+
+lemma [\<phi>reason 2100
+   except \<open> ?Y1 * ?Y2 \<^bold>i\<^bold>m\<^bold>p\<^bold>l\<^bold>i\<^bold>e\<^bold>s ?X \<^bold>a\<^bold>n\<^bold>d ?P @action reason_ToSA ?mode ?G\<close>
+          \<open> 1 \<^bold>i\<^bold>m\<^bold>p\<^bold>l\<^bold>i\<^bold>e\<^bold>s ?X \<^bold>a\<^bold>n\<^bold>d ?P @action reason_ToSA ?mode ?G\<close>
+          \<open> TAIL ?H \<^bold>i\<^bold>m\<^bold>p\<^bold>l\<^bold>i\<^bold>e\<^bold>s ?X \<^bold>a\<^bold>n\<^bold>d ?P @action reason_ToSA ?mode ?G\<close>
+]:
+  " 1 * Y \<^bold>i\<^bold>m\<^bold>p\<^bold>l\<^bold>i\<^bold>e\<^bold>s X \<^bold>a\<^bold>n\<^bold>d P @action reason_ToSA mode G \<Longrightarrow>
+    Y \<^bold>i\<^bold>m\<^bold>p\<^bold>l\<^bold>i\<^bold>e\<^bold>s X \<^bold>a\<^bold>n\<^bold>d P @action reason_ToSA mode G"
+  for X :: \<open>'a::sep_magma_1 set\<close>
+  unfolding mult_1_left .
+
+
+lemma [\<phi>reason 1050 for \<open>?X \<^bold>i\<^bold>m\<^bold>p\<^bold>l\<^bold>i\<^bold>e\<^bold>s \<blangle> ?Y \<brangle> \<^bold>a\<^bold>n\<^bold>d ?P @action reason_ToSA True ?G\<close>
+   except \<open>(?X'::?'a::sep_magma_1 set) \<^bold>i\<^bold>m\<^bold>p\<^bold>l\<^bold>i\<^bold>e\<^bold>s \<blangle> ?Y' \<brangle> \<^bold>a\<^bold>n\<^bold>d ?P @action reason_ToSA True ?G\<close>]:
+  \<open> X \<^bold>i\<^bold>m\<^bold>p\<^bold>l\<^bold>i\<^bold>e\<^bold>s Y \<^bold>a\<^bold>n\<^bold>d P
+\<Longrightarrow> X \<^bold>i\<^bold>m\<^bold>p\<^bold>l\<^bold>i\<^bold>e\<^bold>s \<blangle> Y \<brangle> \<^bold>a\<^bold>n\<^bold>d P @action reason_ToSA True G\<close>
+  \<comment> \<open>If it doesn't have one, it cannot be reasoned by this procedure, so
+      a fallback here handles it.\<close>
+  unfolding FOCUS_TAG_def Action_Tag_def .
+
+
 lemma [\<phi>reason 2000
     for \<open>?R \<^bold>i\<^bold>m\<^bold>p\<^bold>l\<^bold>i\<^bold>e\<^bold>s \<blangle> ?R2 * ?X \<brangle> \<^bold>a\<^bold>n\<^bold>d ?P @action reason_ToSA ?mode ?G\<close>
 (* except \<open>?R \<^bold>i\<^bold>m\<^bold>p\<^bold>l\<^bold>i\<^bold>e\<^bold>s \<blangle> ?R2 * (FIX ?X) \<brangle> \<^bold>a\<^bold>n\<^bold>d ?P @action reason_ToSA ?mode ?G\<close> *)
@@ -1004,7 +1001,6 @@ lemma [\<phi>reason 3200]:
   "R \<^bold>s\<^bold>h\<^bold>i\<^bold>f\<^bold>t\<^bold>s X \<^bold>a\<^bold>n\<^bold>d P @action reason_ToSA mode G \<Longrightarrow>
    R \<heavy_comma> Void \<^bold>s\<^bold>h\<^bold>i\<^bold>f\<^bold>t\<^bold>s X \<^bold>a\<^bold>n\<^bold>d P @action reason_ToSA mode G"
   unfolding mult_1_right .
-
 
 subsection \<open>Subjection\<close>
 
